src/ordered.lean
@@ -1,11 +1,67 @@
 import btree
-import forall_keys
 import tactic.linarith
 set_option pp.generalized_field_notation false
 
-namespace ordered_lemmas
-open btree_def
-open forall_keys_lemmas
+namespace ordered
+open btree
+
+def forall_keys {α : Type} (p : nat → nat → Prop) : nat → btree α → Prop
+| x btree.empty := tt
+| x (btree.node l k a r) :=
+  forall_keys x l ∧ (p x k) ∧ forall_keys x r
+
+
+lemma forall_insert {α : Type} (k k' : nat) (t : btree α) (a : α) (p : nat → nat → Prop) (h₀ : p k' k) :
+  forall_keys p k' t → forall_keys p k' (insert k a t) :=
+begin
+  intro h₁,
+  induction t,
+  case empty {
+    simp only [btree.insert, forall_keys],
+    simp only [forall_keys] at h₁,
+    apply and.intro h₁ (and.intro h₀ h₁)
+  },
+  case node : tl tk ta tr ihl ihr {
+    simp only [btree.insert],
+    simp only [forall_keys] at h₁,
+    by_cases c₁ : (k < tk),
+    { simp only [if_pos c₁, forall_keys], 
+      apply and.intro,
+      { apply ihl, 
+        apply and.left h₁,
+      },
+      { apply and.right h₁ }
+    },
+    { simp only [if_neg c₁],
+      by_cases c₂ : (k > tk),
+      { simp only [if_pos c₂], 
+        simp only [forall_keys],
+        apply and.intro,
+        { apply and.left h₁ },
+        { apply and.intro, 
+          { apply and.left (and.right h₁) },
+          { apply ihr,
+            apply and.right (and.right h₁),
+          }
+        }
+      },
+      { simp only [if_neg c₂, forall_keys],
+        apply and.intro,
+        { apply and.left h₁ },
+        { apply and.intro h₀ (and.right (and.right h₁)), }
+      } 
+    }
+  },
+end
+
+/--
+  A binary tree is ordered when both left and right subtrees of the
+  root node satisfy the predicate that each left subtree has keys
+  less than the root, and each right subtree has keys more than the root.
+-/
+def ordered {α: Type} : btree α → Prop
+| btree.empty := tt
+| (btree.node l k a r) := ordered l ∧ ordered r ∧ (forall_keys (>) k l) ∧ (forall_keys (<) k r)
 
 lemma ordered_insert {α : Type} (t : btree α) (k : nat) (a : α) :
   ordered t → ordered (insert k a t) :=
@@ -13,11 +69,11 @@ begin
   intro h₁,
   induction t,
   case empty {
-    simp only [btree_def.insert, ordered],
+    simp only [btree.insert, ordered],
     finish,
   },
   case node : tl tk ta tr ihl ihr {
-    simp only [btree_def.insert],
+    simp only [btree.insert],
     simp only [ordered] at h₁,
     by_cases c₁ : (k < tk),
     { simp only [if_pos c₁, ordered], 
@@ -68,39 +124,4 @@ begin
   }
 end
 
--- inversion lemmas!
-
-lemma bound_lookup {α : Type} (t : btree α) (k : nat) :
-  bound k t → ∃ (v : α), lookup k t = some v :=
-begin
-  intros h₁,
-  induction t,
-  case empty {
-    simp only [lookup],
-    simp [bound] at h₁,
-    contradiction,
-  },
-  case node : tl tk ta tr ihl ihr {
-    simp only [lookup],
-    by_cases c₁ : (k < tk),
-    { simp only [if_pos c₁],
-      apply ihl,
-      simp only [bound, if_pos c₁] at h₁, 
-      finish,
-    },
-    { simp only [if_neg c₁], 
-      by_cases c₂ : (k > tk),
-      { simp only [if_pos c₂],
-        apply ihr,
-        simp only [bound, if_pos c₂, if_neg c₁] at h₁,
-        finish, 
-      },
-      { simp only [if_neg c₂], 
-        existsi ta,
-        refl,
-      },
-    }
-  }
-end
-
-end ordered_lemmas
+end ordered
